lib/zoo_parabs/ws_queues_public.mli
@@ -1,0 +1,1 @@
+include Ws_queues.S
