lib/zoo_saturn/ws_queue_2.ml
@@ -3,23 +3,23 @@
 *)
 
 type 'a t =
-  'a ref Inf_ws_deque_1.t
+  'a ref Ws_queue_1.t
 
 let create =
-  Inf_ws_deque_1.create
+  Ws_queue_1.create
 
 let push t v =
-  Inf_ws_deque_1.push t (ref v)
+  Ws_queue_1.push t (ref v)
 
 let steal t =
-  match Inf_ws_deque_1.steal t with
+  match Ws_queue_1.steal t with
   | None ->
       None
   | Some slot ->
       Some !slot
 
 let pop t =
-  match Inf_ws_deque_1.pop t with
+  match Ws_queue_1.pop t with
   | None ->
       None
   | Some slot ->
