theories/zoo_saturn/inf_ws_queue_2__code.v
@@ -4,31 +4,31 @@ From zoo.language Require Import
   typeclasses
   notations.
 From zoo_saturn Require Import
-  ws_deque_1.
+  inf_ws_queue_1.
 From zoo_saturn Require Import
-  ws_deque_2__types.
+  inf_ws_queue_2__types.
 From zoo Require Import
   options.
 
-Definition ws_deque_2_create : val :=
-  ws_deque_1_create.
+Definition inf_ws_queue_2_create : val :=
+  inf_ws_queue_1_create.
 
-Definition ws_deque_2_push : val :=
+Definition inf_ws_queue_2_push : val :=
   fun: "t" "v" =>
-    ws_deque_1_push "t" (ref "v").
+    inf_ws_queue_1_push "t" (ref "v").
 
-Definition ws_deque_2_steal : val :=
+Definition inf_ws_queue_2_steal : val :=
   fun: "t" =>
-    match: ws_deque_1_steal "t" with
+    match: inf_ws_queue_1_steal "t" with
     | None =>
         §None
     | Some "slot" =>
         ‘Some( !"slot" )
     end.
 
-Definition ws_deque_2_pop : val :=
+Definition inf_ws_queue_2_pop : val :=
   fun: "t" =>
-    match: ws_deque_1_pop "t" with
+    match: inf_ws_queue_1_pop "t" with
     | None =>
         §None
     | Some "slot" =>
