theories/zoo_parabs/ws_queues_private__types.v
@@ -13,61 +13,61 @@ From zoo Require Import
   options.
 
 Notation "'Blocked'" := (
-  in_type "zoo_parabs.ws_deques_private.status" 0
+  in_type "zoo_parabs.ws_queues_private.status" 0
 )(in custom zoo_tag
 ).
 Notation "'Nonblocked'" := (
-  in_type "zoo_parabs.ws_deques_private.status" 1
+  in_type "zoo_parabs.ws_queues_private.status" 1
 )(in custom zoo_tag
 ).
 
 Notation "'RequestBlocked'" := (
-  in_type "zoo_parabs.ws_deques_private.request" 0
+  in_type "zoo_parabs.ws_queues_private.request" 0
 )(in custom zoo_tag
 ).
 Notation "'RequestNone'" := (
-  in_type "zoo_parabs.ws_deques_private.request" 1
+  in_type "zoo_parabs.ws_queues_private.request" 1
 )(in custom zoo_tag
 ).
 Notation "'RequestSome'" := (
-  in_type "zoo_parabs.ws_deques_private.request" 2
+  in_type "zoo_parabs.ws_queues_private.request" 2
 )(in custom zoo_tag
 ).
 
 Notation "'ResponseWaiting'" := (
-  in_type "zoo_parabs.ws_deques_private.response" 0
+  in_type "zoo_parabs.ws_queues_private.response" 0
 )(in custom zoo_tag
 ).
 Notation "'ResponseNone'" := (
-  in_type "zoo_parabs.ws_deques_private.response" 1
+  in_type "zoo_parabs.ws_queues_private.response" 1
 )(in custom zoo_tag
 ).
 Notation "'ResponseSome'" := (
-  in_type "zoo_parabs.ws_deques_private.response" 2
+  in_type "zoo_parabs.ws_queues_private.response" 2
 )(in custom zoo_tag
 ).
 
 Notation "'size'" := (
-  in_type "zoo_parabs.ws_deques_private.t" 0
+  in_type "zoo_parabs.ws_queues_private.t" 0
 )(in custom zoo_field
 ).
 Notation "'deques'" := (
-  in_type "zoo_parabs.ws_deques_private.t" 1
+  in_type "zoo_parabs.ws_queues_private.t" 1
 )(in custom zoo_field
 ).
 Notation "'statuses'" := (
-  in_type "zoo_parabs.ws_deques_private.t" 2
+  in_type "zoo_parabs.ws_queues_private.t" 2
 )(in custom zoo_field
 ).
 Notation "'requests'" := (
-  in_type "zoo_parabs.ws_deques_private.t" 3
+  in_type "zoo_parabs.ws_queues_private.t" 3
 )(in custom zoo_field
 ).
 Notation "'responses'" := (
-  in_type "zoo_parabs.ws_deques_private.t" 4
+  in_type "zoo_parabs.ws_queues_private.t" 4
 )(in custom zoo_field
 ).
 Notation "'force_mutable'" := (
-  in_type "zoo_parabs.ws_deques_private.t" 5
+  in_type "zoo_parabs.ws_queues_private.t" 5
 )(in custom zoo_field
 ).
