theories/zoo_parabs/ws_queues_public.v
@@ -1,0 +1,469 @@
+From zoo Require Import
+  prelude.
+From zoo.iris.bi Require Import
+  big_op.
+From zoo.language Require Import
+  notations.
+From zoo.diaframe Require Import
+  diaframe.
+From zoo_std Require Import
+  option
+  array
+  random_round.
+From zoo_saturn Require Import
+  ws_queue_2.
+From zoo_parabs Require Export
+  base
+  ws_queues_public__code.
+From zoo Require Import
+  options.
+
+Implicit Types v t queue round : val.
+Implicit Types vs queues : list val.
+Implicit Types vss : list (list val).
+Implicit Types status : status.
+
+Class WsQueuesPublicG Σ `{zoo_G : !ZooG Σ} := {
+  #[local] ws_queues_public_G_ws_queue_G :: WsQueue2G Σ ;
+}.
+
+Definition ws_queues_public_Σ := #[
+  ws_queue_2_Σ
+].
+#[global] Instance subG_ws_queues_public_Σ Σ `{zoo_G : !ZooG Σ} :
+  subG ws_queues_public_Σ Σ →
+  WsQueuesPublicG Σ.
+Proof.
+  solve_inG.
+Qed.
+
+Section ws_queues_public_G.
+  Context `{ws_queues_public_G : WsQueuesPublicG Σ}.
+
+  Definition ws_queues_public_inv t ι sz : iProp Σ :=
+    ∃ queues,
+    ⌜sz = length queues⌝ ∗
+    array_model t DfracDiscarded queues ∗
+    [∗ list] queue ∈ queues,
+      ws_queue_2_inv queue ι.
+  #[local] Instance : CustomIpatFormat "inv" :=
+    "(
+      %queues{} &
+      %Hqueues{}_length &
+      #Hqueues{} &
+      #Hqueues{}_inv
+    )".
+
+  Definition ws_queues_public_model t vss : iProp Σ :=
+    ∃ queues,
+    array_model t DfracDiscarded queues ∗
+    [∗ list] i ↦ queue; vs ∈ queues; vss,
+      ws_queue_2_model queue vs.
+  #[local] Instance : CustomIpatFormat "model" :=
+    "(
+      %queues_ &
+      Hqueues_ &
+      Hqueues_model
+    )".
+
+  Definition ws_queues_public_owner t i status : iProp Σ :=
+    ∃ queues queue,
+    ⌜queues !! i = Some queue⌝ ∗
+    array_model t DfracDiscarded queues ∗
+    ws_queue_2_owner queue.
+  #[local] Instance : CustomIpatFormat "owner" :=
+    "(
+      %queues{=_} &
+      %queue{} &
+      %Hqueues{}_lookup &
+      Hqueues{=_} &
+      Hqueue{}_owner
+    )".
+
+  #[global] Instance ws_queues_public_model_timeless t vss :
+    Timeless (ws_queues_public_model t vss).
+  Proof.
+    apply _.
+  Qed.
+  #[global] Instance ws_queues_public_inv_persistent t ι sz :
+    Persistent (ws_queues_public_inv t ι sz).
+  Proof.
+    apply _.
+  Qed.
+
+  Lemma ws_queues_public_inv_agree t ι sz1 sz2 :
+    ws_queues_public_inv t ι sz1 -∗
+    ws_queues_public_inv t ι sz2 -∗
+    ⌜sz1 = sz2⌝.
+  Proof.
+    iIntros "(:inv =1) (:inv =2)".
+    iDestruct (array_model_agree with "Hqueues1 Hqueues2") as %<-.
+    iSteps.
+  Qed.
+
+  Lemma ws_queues_public_inv_owner t ι sz i status :
+    ws_queues_public_inv t ι sz -∗
+    ws_queues_public_owner t i status -∗
+    ⌜i < sz⌝.
+  Proof.
+    iIntros "(:inv) (:owner)".
+    iDestruct (array_model_agree with "Hqueues Hqueues_") as %<-. iClear "Hqueues_".
+    iPureIntro. rewrite Hqueues_length. eapply lookup_lt_Some. done.
+  Qed.
+  Lemma ws_queues_public_owner_exclusive t i status1 status2 :
+    ws_queues_public_owner t i status1 -∗
+    ws_queues_public_owner t i status2 -∗
+    False.
+  Proof.
+    iIntros "(:owner =1) (:owner =2)".
+    iDestruct (array_model_agree with "Hqueues1 Hqueues2") as %<-. iClear "Hqueues2".
+    simplify.
+    iApply (ws_queue_2_owner_exclusive with "Hqueue1_owner Hqueue2_owner").
+  Qed.
+
+  Lemma ws_queues_public_create_spec ι sz :
+    (0 ≤ sz)%Z →
+    {{{
+      True
+    }}}
+      ws_queues_public_create #sz
+    {{{ t,
+      RET t;
+      ws_queues_public_inv t ι ₊sz ∗
+      ws_queues_public_model t (replicate ₊sz []) ∗
+      [∗ list] i ∈ seq 0 ₊sz,
+        ws_queues_public_owner t i Nonblocked
+    }}}.
+  Proof.
+    iIntros "%Hsz %Φ _ HΦ".
+
+    wp_rec.
+
+    pose (Ψ (_ : nat) queues := (
+      ( [∗ list] queue ∈ queues,
+        ws_queue_2_inv queue ι
+      ) ∗
+      ( [∗ list] queue ∈ queues,
+        ws_queue_2_model queue []
+      ) ∗
+      ( [∗ list] queue ∈ queues,
+        ws_queue_2_owner queue
+      )
+    )%I).
+    iApply wp_fupd.
+    wp_smart_apply (array_unsafe_init_spec Ψ) as (t queues) "(%Hqueues_length & Hqueues & (Hinv & Hmodel & Howner))"; first done.
+    { iSteps.
+      wp_apply (ws_queue_2_create_spec with "[//]").
+      rewrite /Ψ. setoid_rewrite big_sepL_snoc. iSteps.
+    }
+    iMod (array_model_persist with "Hqueues") as "#Hqueues".
+
+    iApply "HΦ". iSplitL "Hinv"; last iSplitL "Hmodel".
+    - iExists queues. iSteps.
+    - iExists queues. rewrite big_sepL2_replicate_r //. iSteps.
+    - rewrite big_sepL_seq_index //.
+      iApply (big_sepL_impl with "Howner").
+      iSteps.
+  Qed.
+
+  Lemma ws_queues_public_size_spec t ι sz :
+    {{{
+      ws_queues_public_inv t ι sz
+    }}}
+      ws_queues_public_size t
+    {{{
+      RET #sz;
+      True
+    }}}.
+  Proof.
+    iSteps.
+    wp_apply array_size_spec; iSteps.
+  Qed.
+
+  Lemma ws_queues_public_block_spec t ι sz i i_ :
+    i = ⁺i_ →
+    {{{
+      ws_queues_public_inv t ι sz ∗
+      ws_queues_public_owner t i_ Nonblocked
+    }}}
+      ws_queues_public_block t #i
+    {{{
+      RET ();
+      ws_queues_public_owner t i_ Blocked
+    }}}.
+  Proof.
+    iSteps.
+  Qed.
+
+  Lemma ws_queues_public_unblock_spec t ι sz i i_ :
+    i = ⁺i_ →
+    {{{
+      ws_queues_public_inv t ι sz ∗
+      ws_queues_public_owner t i_ Blocked
+    }}}
+      ws_queues_public_unblock t #i
+    {{{
+      RET ();
+      ws_queues_public_owner t i_ Nonblocked
+    }}}.
+  Proof.
+    iSteps.
+  Qed.
+
+  Lemma ws_queues_public_push_spec t ι sz i i_ v :
+    i = ⁺i_ →
+    <<<
+      ws_queues_public_inv t ι sz ∗
+      ws_queues_public_owner t i_ Nonblocked
+    | ∀∀ vss,
+      ws_queues_public_model t vss
+    >>>
+      ws_queues_public_push t #i v @ ↑ι
+    <<<
+      ∃∃ vs,
+      ⌜vss !! i_ = Some vs⌝ ∗
+      ws_queues_public_model t (<[i_ := vs ++ [v]]> vss)
+    | RET ();
+      ws_queues_public_owner t i_ Nonblocked
+    >>>.
+  Proof.
+    iIntros (->) "%Φ ((:inv) & (:owner)) HΦ".
+    iDestruct (array_model_agree with "Hqueues Hqueues_") as %<-. iClear "Hqueues_".
+
+    wp_rec.
+    wp_smart_apply (array_unsafe_get_spec with "Hqueues") as "_"; [lia | done | lia |].
+
+    iDestruct (big_sepL_lookup with "Hqueues_inv") as "Hqueue_inv"; first done.
+    awp_smart_apply (ws_queue_2_push_spec with "[$Hqueue_inv $Hqueue_owner]").
+    iApply (aacc_aupd_commit with "HΦ"); first done. iIntros "%vss (:model)".
+    iDestruct (array_model_agree with "Hqueues Hqueues_") as %<-. iClear "Hqueues_".
+    iDestruct (big_sepL2_lookup_Some_l with "Hqueues_model") as %(vs & Hvss_lookup); first done.
+    iDestruct (big_sepL2_insert_acc with "Hqueues_model") as "(Hqueue_model & Hqueues_model)"; [done.. |].
+    iAaccIntro with "Hqueue_model".
+    all: iIntros "Hqueue_model".
+    all: iDestruct ("Hqueues_model" with "Hqueue_model") as "Hqueues_model".
+    - rewrite !list_insert_id //. iSteps.
+    - rewrite list_insert_id //. iSteps.
+  Qed.
+
+  Lemma ws_queues_public_pop_spec t ι sz i i_ :
+    i = ⁺i_ →
+    <<<
+      ws_queues_public_inv t ι sz ∗
+      ws_queues_public_owner t i_ Nonblocked
+    | ∀∀ vss,
+      ws_queues_public_model t vss
+    >>>
+      ws_queues_public_pop t #i @ ↑ι
+    <<<
+      ∃∃ o,
+      match o with
+      | None =>
+          ⌜vss !! i_ = Some []⌝ ∗
+          ws_queues_public_model t vss
+      | Some v =>
+          ∃ vs,
+          ⌜vss !! i_ = Some (vs ++ [v])⌝ ∗
+          ws_queues_public_model t (<[i_ := vs]> vss)
+      end
+    | RET o;
+      ws_queues_public_owner t i_ Nonblocked
+    >>>.
+  Proof.
+    iIntros (->) "%Φ ((:inv) & (:owner)) HΦ".
+    iDestruct (array_model_agree with "Hqueues Hqueues_") as %<-. iClear "Hqueues_".
+
+    wp_rec.
+    wp_smart_apply (array_unsafe_get_spec with "Hqueues") as "_"; [lia | done | lia |].
+
+    iDestruct (big_sepL_lookup with "Hqueues_inv") as "Hqueue_inv"; first done.
+    awp_smart_apply (ws_queue_2_pop_spec with "[$Hqueue_inv $Hqueue_owner]").
+    iApply (aacc_aupd_commit with "HΦ"); first done. iIntros "%vss (:model)".
+    iDestruct (array_model_agree with "Hqueues Hqueues_") as %<-. iClear "Hqueues_".
+    iDestruct (big_sepL2_lookup_Some_l with "Hqueues_model") as %(vs & Hvss_lookup); first done.
+    iDestruct (big_sepL2_insert_acc with "Hqueues_model") as "(Hqueue_model & Hqueues_model)"; [done.. |].
+    iAaccIntro with "Hqueue_model".
+
+    - iIntros "Hqueue_model".
+      iDestruct ("Hqueues_model" with "Hqueue_model") as "Hqueues_model".
+      rewrite !list_insert_id //. iSteps.
+
+    - iIntros "%o Hqueue_model". iExists o. iSplitL; last iSteps. destruct o as [v |].
+
+      + iDestruct "Hqueue_model" as "(%vs' & -> & Hqueue_model)".
+        iDestruct ("Hqueues_model" with "Hqueue_model") as "Hqueues_model".
+        rewrite list_insert_id //. iSteps.
+
+      + iDestruct "Hqueue_model" as "(-> & Hqueue_model)".
+        iDestruct ("Hqueues_model" with "Hqueue_model") as "Hqueues_model".
+        rewrite !list_insert_id //. iSteps.
+  Qed.
+
+  Lemma ws_queues_public_steal_to_spec t ι (sz : nat) i i_ j :
+    i = ⁺i_ →
+    (0 ≤ j < sz)%Z →
+    <<<
+      ws_queues_public_inv t ι sz ∗
+      ws_queues_public_owner t i_ Blocked
+    | ∀∀ vss,
+      ws_queues_public_model t vss
+    >>>
+      ws_queues_public_steal_to t #i #j @ ↑ι
+    <<<
+      ∃∃ o,
+      match o with
+      | None =>
+          ws_queues_public_model t vss
+      | Some v =>
+          ∃ vs,
+          ⌜vss !! ₊j = Some (v :: vs)⌝ ∗
+          ws_queues_public_model t (<[₊j := vs]> vss)
+      end
+    | RET o;
+      ws_queues_public_owner t i_ Blocked
+    >>>.
+  Proof.
+    iIntros (-> Hj) "%Φ ((:inv) & Howner) HΦ".
+
+    wp_rec.
+    destruct (lookup_lt_is_Some_2 queues ₊j) as (queue & Hqueue_lookup); first lia.
+    wp_smart_apply (array_unsafe_get_spec with "Hqueues") as "_"; [lia | done.. |].
+
+    iDestruct (big_sepL_lookup with "Hqueues_inv") as "#Hqueue_inv"; first done.
+    awp_smart_apply (ws_queue_2_steal_spec with "Hqueue_inv") without "Howner".
+    iApply (aacc_aupd_commit with "HΦ"); first done. iIntros "%vss (:model)".
+    iDestruct (array_model_agree with "Hqueues Hqueues_") as %<-. iClear "Hqueues_".
+    iDestruct (big_sepL2_lookup_Some_l with "Hqueues_model") as %(vs & Hvss_lookup); first done.
+    iDestruct (big_sepL2_insert_acc with "Hqueues_model") as "(Hqueue_model & Hqueues_model)"; [done.. |].
+    iAaccIntro with "Hqueue_model".
+
+    - iIntros "Hqueue_model".
+      iDestruct ("Hqueues_model" with "Hqueue_model") as "Hqueues_model".
+      rewrite !list_insert_id //. iSteps.
+
+    - iIntros "Hqueue_model !>". destruct vs as [| v vs].
+
+      + iExists None. iSplitL; last iSteps.
+        iDestruct ("Hqueues_model" with "Hqueue_model") as "Hqueues_model".
+        rewrite !list_insert_id //. iSteps.
+
+      + iExists (Some v). iSplitL; last iSteps.
+        iDestruct ("Hqueues_model" with "Hqueue_model") as "Hqueues_model".
+        rewrite list_insert_id //. iSteps.
+  Qed.
+End ws_queues_public_G.
+
+#[global] Opaque ws_queues_public_inv.
+#[global] Opaque ws_queues_public_model.
+#[global] Opaque ws_queues_public_owner.
+
+Section ws_queues_public_G.
+  Context `{ws_queues_public_G : WsQueuesPublicG Σ}.
+
+  #[local] Lemma ws_queues_public_steal_as_0_spec t ι (sz : nat) i i_ round (n : nat) :
+    i = ⁺i_ →
+    <<<
+      ws_queues_public_inv t ι sz ∗
+      ws_queues_public_owner t i_ Blocked ∗
+      random_round_model' round (sz - 1) n
+    | ∀∀ vss,
+      ws_queues_public_model t vss
+    >>>
+      ws_queues_public_steal_as_0 t #sz #i round #n @ ↑ι
+    <<<
+      ∃∃ o,
+      match o with
+      | None =>
+          ws_queues_public_model t vss
+      | Some v =>
+          ∃ j vs,
+          ⌜₊i ≠ j⌝ ∗
+          ⌜vss !! j = Some (v :: vs)⌝ ∗
+          ws_queues_public_model t (<[j := vs]> vss)
+      end
+    | RET o;
+      ∃ n,
+      ws_queues_public_owner t i_ Blocked ∗
+      random_round_model' round (sz - 1) n
+    >>>.
+  Proof.
+    iIntros (->) "%Φ (#Hinv & Howner & Hround) HΦ".
+    iDestruct (ws_queues_public_inv_owner with "Hinv Howner") as %Hi.
+
+    iLöb as "HLöb" forall (n).
+
+    wp_rec. wp_pures.
+    case_bool_decide as Hcase; wp_pures.
+
+    - iMod "HΦ" as "(%vss & Hmodel & _ & HΦ)".
+      iApply ("HΦ" $! None with "Hmodel [$Howner Hround]"); first iSteps.
+
+    - wp_apply (random_round_next_spec' with "Hround") as (j) "(%Hj & Hround)"; first lia.
+      wp_pures.
+      rewrite Nat2Z.id.
+      pose k := (i_ + 1 + j) `mod` sz.
+      assert ((i_ + 1 + j) `rem` sz = k)%Z as ->.
+      { rewrite Z.rem_mod_nonneg; lia. }
+      awp_smart_apply (ws_queues_public_steal_to_spec with "[$Hinv $Howner]") without "Hround"; [done | lia |].
+      iApply (aacc_aupd with "HΦ"); first done. iIntros "%vss Hmodel".
+      iAaccIntro with "Hmodel"; first iSteps. iIntros ([ v |]).
+
+      + rewrite Nat2Z.id.
+        iSteps as (vs Hlookup) "Hmodel". iExists (Some v). iSteps. iExists k. iSteps. iPureIntro.
+        clear Hlookup. rewrite {}/k.
+        destruct (decide (i_ + 1 + j < sz)).
+        * rewrite Nat.mod_small //. lia.
+        * assert (i_ + 1 + j < sz * 2) as ?%Nat.div_lt_upper_bound by lia; last lia.
+          assert ((i_ + 1 + j) `div` sz = 1) by lia.
+          lia.
+
+      + iSteps as "HΦ Howner Hround".
+        assert (n - 1 = (n - 1)%nat)%Z as -> by lia.
+        iSteps.
+  Qed.
+  Lemma ws_queues_public_steal_as_spec t ι sz i i_ round :
+    i = ⁺i_ →
+    0 < sz →
+    <<<
+      ws_queues_public_inv t ι sz ∗
+      ws_queues_public_owner t i_ Blocked ∗
+      random_round_model' round (sz - 1) (sz - 1)
+    | ∀∀ vss,
+      ws_queues_public_model t vss
+    >>>
+      ws_queues_public_steal_as t #i round @ ↑ι
+    <<<
+      ∃∃ o,
+      match o with
+      | None =>
+          ws_queues_public_model t vss
+      | Some v =>
+          ∃ j vs,
+          ⌜₊i ≠ j⌝ ∗
+          ⌜vss !! j = Some (v :: vs)⌝ ∗
+          ws_queues_public_model t (<[j := vs]> vss)
+      end
+    | RET o;
+      ∃ n,
+      ws_queues_public_owner t i_ Blocked ∗
+      random_round_model' round (sz - 1) n
+    >>>.
+  Proof.
+    iIntros (->) "%Hsz %Φ (#Hinv & Hround) HΦ".
+
+    wp_rec.
+    wp_smart_apply (ws_queues_public_size_spec with "Hinv") as "_".
+    wp_pures.
+    assert (sz - 1 = (sz - 1)%nat)%Z as -> by lia.
+    wp_apply (ws_queues_public_steal_as_0_spec with "[$Hinv $Hround] HΦ"); first done.
+  Qed.
+End ws_queues_public_G.
+
+#[global] Opaque ws_queues_public_create.
+#[global] Opaque ws_queues_public_size.
+#[global] Opaque ws_queues_public_block.
+#[global] Opaque ws_queues_public_unblock.
+#[global] Opaque ws_queues_public_push.
+#[global] Opaque ws_queues_public_pop.
+#[global] Opaque ws_queues_public_steal_to.
+#[global] Opaque ws_queues_public_steal_as.
