theories/zoo_parabs/ws_queues_public__code.v
@@ -1,0 +1,63 @@
+From zoo Require Import
+  prelude.
+From zoo.language Require Import
+  typeclasses
+  notations.
+From zoo_std Require Import
+  array
+  random_round.
+From zoo_saturn Require Import
+  ws_queue_2.
+From zoo_parabs Require Import
+  ws_queues_public__types.
+From zoo Require Import
+  options.
+
+Definition ws_queues_public_create : val :=
+  fun: "sz" =>
+    array_unsafe_init "sz" ws_queue_2_create.
+
+Definition ws_queues_public_size : val :=
+  array_size.
+
+Definition ws_queues_public_block : val :=
+  fun: "_t" "_i" =>
+    ().
+
+Definition ws_queues_public_unblock : val :=
+  fun: "_t" "_i" =>
+    ().
+
+Definition ws_queues_public_push : val :=
+  fun: "t" "i" "v" =>
+    let: "queue" := array_unsafe_get "t" "i" in
+    ws_queue_2_push "queue" "v".
+
+Definition ws_queues_public_pop : val :=
+  fun: "t" "i" =>
+    let: "queue" := array_unsafe_get "t" "i" in
+    ws_queue_2_pop "queue".
+
+Definition ws_queues_public_steal_to : val :=
+  fun: "t" "_i" "j" =>
+    let: "queue" := array_unsafe_get "t" "j" in
+    ws_queue_2_steal "queue".
+
+Definition ws_queues_public_steal_as_0 : val :=
+  rec: "steal_as" "t" "sz" "i" "round" "n" =>
+    if: "n" ≤ #0 then (
+      §None
+    ) else (
+      let: "j" := ("i" + #1 + random_round_next "round") `rem` "sz" in
+      match: ws_queues_public_steal_to "t" "i" "j" with
+      | None =>
+          "steal_as" "t" "sz" "i" "round" ("n" - #1)
+      |_ as "res" =>
+          "res"
+      end
+    ).
+
+Definition ws_queues_public_steal_as : val :=
+  fun: "t" "i" "round" =>
+    let: "sz" := ws_queues_public_size "t" in
+    ws_queues_public_steal_as_0 "t" "sz" "i" "round" ("sz" - #1).
