theories/zoo_saturn/ws_queue_1.v
@@ -1,0 +1,142 @@
+From zoo Require Import
+  prelude.
+From zoo.language Require Import
+  notations.
+From zoo.diaframe Require Import
+  diaframe.
+From zoo_std Require Import
+  option.
+From zoo_saturn Require Export
+  base
+  ws_queue_1__code.
+From zoo_saturn Require Import
+  ws_queue_1__types.
+From zoo Require Import
+  options.
+
+Implicit Types v t : val.
+Implicit Types vs : list val.
+
+Class WsQueue1G Σ `{zoo_G : !ZooG Σ} := {
+}.
+
+Definition ws_queue_1_Σ := #[
+].
+#[global] Instance subG_ws_queue_1_Σ Σ `{zoo_G : !ZooG Σ} :
+  subG ws_queue_1_Σ Σ →
+  WsQueue1G Σ .
+Proof.
+  (* solve_inG. *)
+Qed.
+
+Section ws_queue_1_G.
+  Context `{ws_queue_1_G : WsQueue1G Σ}.
+
+  Definition ws_queue_1_inv t (ι : namespace) : iProp Σ.
+  Proof. Admitted.
+
+  Definition ws_queue_1_model t vs : iProp Σ.
+  Proof. Admitted.
+
+  Definition ws_queue_1_owner t : iProp Σ.
+  Proof. Admitted.
+
+  #[global] Instance ws_queue_1_model_timeless t model :
+    Timeless (ws_queue_1_model t model).
+  Proof.
+  Admitted.
+  #[global] Instance ws_queue_1_owner_timeless t :
+    Timeless (ws_queue_1_owner t).
+  Proof.
+  Admitted.
+  #[global] Instance ws_queue_1_inv_persistent t ι :
+    Persistent (ws_queue_1_inv t ι).
+  Proof.
+  Admitted.
+
+  Lemma ws_queue_1_owner_exclusive t :
+    ws_queue_1_owner t -∗
+    ws_queue_1_owner t -∗
+    False.
+  Proof.
+  Admitted.
+
+  Lemma ws_queue_1_create_spec ι :
+    {{{
+      True
+    }}}
+      ws_queue_1_create ()
+    {{{ t,
+      RET t;
+      ws_queue_1_inv t ι ∗
+      ws_queue_1_model t [] ∗
+      ws_queue_1_owner t
+    }}}.
+  Proof.
+  Admitted.
+
+  Lemma ws_queue_1_push_spec t ι v :
+    <<<
+      ws_queue_1_inv t ι ∗
+      ws_queue_1_owner t
+    | ∀∀ vs,
+      ws_queue_1_model t vs
+    >>>
+      ws_queue_1_push t v @ ↑ι
+    <<<
+      ws_queue_1_model t (vs ++ [v])
+    | RET ();
+      ws_queue_1_owner t
+    >>>.
+  Proof.
+  Admitted.
+
+  Lemma ws_queue_1_steal_spec t ι :
+    <<<
+      ws_queue_1_inv t ι
+    | ∀∀ vs,
+      ws_queue_1_model t vs
+    >>>
+      ws_queue_1_steal t @ ↑ι
+    <<<
+      ws_queue_1_model t (tail vs)
+    | RET head vs;
+      True
+    >>>.
+  Proof.
+  Admitted.
+
+  Lemma ws_queue_1_pop_spec t ι :
+    <<<
+      ws_queue_1_inv t ι ∗
+      ws_queue_1_owner t
+    | ∀∀ vs,
+      ws_queue_1_model t vs
+    >>>
+      ws_queue_1_pop t @ ↑ι
+    <<<
+      ∃∃ o,
+      match o with
+      | None =>
+          ⌜vs = []⌝ ∗
+          ws_queue_1_model t []
+      | Some v =>
+          ∃ vs',
+          ⌜vs = vs' ++ [v]⌝ ∗
+          ws_queue_1_model t vs'
+      end
+    | RET o;
+      ws_queue_1_owner t
+    >>>.
+  Proof.
+  Admitted.
+End ws_queue_1_G.
+
+#[global] Opaque ws_queue_1_create.
+#[global] Opaque ws_queue_1_push.
+#[global] Opaque ws_queue_1_pop.
+#[global] Opaque ws_queue_1_steal.
+
+#[global] Opaque ws_queue_1_inv.
+#[global] Opaque ws_queue_1_model.
+#[global] Opaque ws_queue_1_owner.
