theories/zoo_saturn/ws_queue_2__types.v
@@ -4,7 +4,7 @@ From zoo.language Require Import
   typeclasses
   notations.
 From zoo_saturn Require Import
-  ws_deque_1.
+  ws_queue_1.
 From zoo Require Import
   options.
 
